---
layout: problemset_topology_munkres2e
title: Section 67 Direct Sums of Abelian Groups
description: This section defines direct sums and free abelian groups.
parent: Chapter 11 The Seifert-van Kampen Theorem
grand_parent: Topology, Munkres 2e Solutions
permalink: topology_munkres_solutions/section67
nav_order: 67
---

* TOC
{:toc}

---

<div class='problem_stmt completed' markdown='1'>

### Problem 67.1
Suppose that $G = \sum{G_\alpha}$. Show this sum is direct if and only if the equation

$$ x_{\alpha_1} + \cdots + x_{\alpha_n} = 0 $$

implies that $x_{\alpha_i}$ equals 0. *(Here, $x_{\alpha_i} \in G_{\alpha_i}$ and the indices are distinct.)*

{: .no_toc}
#### Proof.
Let $J$ be the indexing set for $G_\alpha$. That is, $\set{G_\alpha} = \set{G_\alpha}_{\alpha \in J}$.

For the forward direction, assume that $G$ is a direct sum of subgroups $G_{\alpha}$. Therefore, for all $g \in G$, there is a unique $J$-tuple that sums up to $g$. Let $(x_{\alpha_i})_{i=1}^{n} \in \set{G\_\alpha}$ for some $n \in \N$ such that $S := \sum\_{i=1}^{n}{x\_{\alpha_i}} = 0$. Observe that $(0, \dots, 0)$ is a $J$-tuple that satisfies $S$. Since $G$ is a direct sum and $J$-tuple representations are unique, $S = 0$ implies that $(x\_{\alpha_i})\_{i=1}^{n} = (0)$.

For the backwards direction, assume that for all $J$-tuples $(x_{\alpha_i})_{i=1}^{n}$, $\sum\_{i=1}^{n}{x\_{\alpha_i}} = 0$ implies that $(x\_{\alpha_i})\_{i=1}^{n} = (0)$. WTS that $J$-tuple representations are unique.

Let $x \in G$ and let $(a_\alpha)_{\alpha \in J}$ and $(b\_\alpha)\_{\alpha \in J}$ be two $J$-tuples that represent $x$. Then, $a\_\alpha = 0$ and $b\_\alpha = 0$ for all but finitely many $\alpha$'s. Then, we can relabel $(a\_\alpha)$ as $(a\_{\alpha_i})\_{i=1}^{n}$ by removing all $\alpha \in J$ such that $a\_\alpha = 0$. Similarly for $(b\_\alpha)$ as $(b\_{\beta_i})\_{i=1}^{m}$. Then, for some $k \in \N$ with $n,m \leq k \leq n+m$, we can relabel $(a\_\alpha)$ and $(b\_\alpha)$ as $(a\_{\gamma_i})\_{i=1}^{k}$ and $(b\_{\gamma_i})\_{i=1}^{k}$ where $\set{\alpha_i}, \set{\beta_i} \subseteq \set{\gamma_i}$. Observe that for some $\gamma_i$'s, $a\_{\gamma_i} = 0$ or $b\_{\gamma_i} = 0$.

Then, $x - x = 0$ can be represented by $(a\_{\gamma_i})\_{i=1}^{k} - (b\_{\gamma_i})\_{i=1}^{k} = (a\_{\gamma_i} - b\_{\gamma_i})\_{i=1}^{k}$. By assumption, for all $i = 1, \dots, k$, $a_{\gamma_i} - b_{\gamma_i} = 0$. Equivalently, $a_{\gamma_i} = b_{\gamma_i}$.

Since for all $\alpha \not\in \set{\gamma_i}$, $a_\alpha = 0$ and $b_\alpha = 0$, $(a_\alpha)\_{\alpha \in J} = (b\_\alpha)_{\alpha \in J}$. Therefore, $G$ is a direct sum.
</div>

---

<div class='problem_stmt completed' markdown='1'>

### Problem 67.2
Show that if $G_1$ is a subgroup of $G$, there may be no subgroup $G_2$ of $G$ such that $G = G_1 \oplus G_2$. *[Hint: Set $G = \Z$ and $G_1 = 2\Z$.]*

{: .no_toc}
#### Answer.
Set $G = \Z$ and $G_1 = 2\Z$. Assume, FTSOC, that there exists $G_2 \subset G$ such that $G = G_1 \oplus G_2$.

By Corollary 67.3, $G / G_2 \cong G_1$ and $G / G_1 \cong G_2$.
We'll use the second isomorphism. Therefore, $\Z / 2\Z \cong G_2$ and $G = 2\Z \oplus \Z_2$.

Let $x = (0,1+2\Z) \in G_1 \oplus G_2$. Then, $2(x) = 2(0,1+2\Z) = (0,2\Z) = 0 \in G_1 \oplus G_2$. Therefore, $x$ has order $2$. However, $G = \Z$ has no element of order $2$. Contradiction.

</div>

---

<div class='problem_stmt has_issues' markdown='1'>

### Problem 67.3
If $G$ is free abelian with basis $\set{x,y}$, show that $\set{2x+3y, x-y}$ is also a basis for $G$.

<div class='problem_notes' markdown='1'>
There may be a typo to this problem. The $\set{2x+3y, x-y}$ is not a basis for $G$ but is a basis for an isomorphic copy of $G$.

Reference: (1) [this StackExchange post.](https://math.stackexchange.com/questions/211625/let-x-y-be-the-basis-of-a-free-abelian-group-of-rank-2-prove-that-2x3y)
</div>

{: .no_toc}
#### Proof, with typo fixed.
Assume that $G$ is free abelian with basis $\set{x,y}$. WTS that $\set{2x+3y, x+y}$ is also a basis for $G$. Let $H_1 = \ket{2x + 3y}$ and $H_2 = \ket{x+y}$, the groups generated by $2x+3y$ and $x+y$ respectively.

1. WTS that $H_1$ and $H_2$ are infinite cyclic groups.
   1. Let $n \in \Z$ such that $n(2x+3y)=0$.
      Then, $2nx + 3ny = 0$. By Problem 67.1 and since $G = H_1 \oplus H_2$, then $2n = 0$ and $3n = 0$. Thus, $n=0$. Therefore, $|2x+3y| = \infty$.
   2. Let $n \in \Z$ such that $n(x+y)=0$. As with $H_1$, $n=0$.
      Therefore, $|x+y| = \infty$.
2. WTS that $G = H_1 + H_2$. <span class='note'> This is where $x-y$ fails. </span>
   1. Let $r, s \in \Z$ with $(r)(2x+3y) + (s)(x+y) = x$.
      Then,

      $$
          (2r+s)x + (3r+s)y = x
          \implies
                \begin{pmatrix} 2 & 1 \\ 3 & 1 \end{pmatrix}
                \begin{pmatrix} r \\ s \end{pmatrix}
                =
                \begin{pmatrix} 1 \\ 0 \end{pmatrix}
          \\ \implies
                \begin{pmatrix} r \\ s \end{pmatrix}
                =
                \begin{pmatrix} 2 & 1 \\ 3 & 1 \end{pmatrix}^{-1}
                \begin{pmatrix} 1 \\ 0 \end{pmatrix}
          =
                \frac{1}{-1}\begin{pmatrix} 1 & -1 \\ -3 & 2 \end{pmatrix}
                \begin{pmatrix} 1 \\ 0 \end{pmatrix}
                =
                \begin{pmatrix} -1 \\ 3 \end{pmatrix}.
      $$

      Therefore, $x = (-1)(2x+3y) + (3)(x+y)$.

   2. Let $r, s \in \Z$ with $(r)(2x+2y) + (s)(x+y) = y$.
      Then,

      $$
          (2r+s)x + (3r+s)y = y
          \implies
                \begin{pmatrix} 2 & 1 \\ 3 & 1 \end{pmatrix}
                \begin{pmatrix} r \\ s \end{pmatrix}
                =
                \begin{pmatrix} 0 \\ 1 \end{pmatrix}
          \\ \implies
                \begin{pmatrix} r \\ s \end{pmatrix}
                =
                \begin{pmatrix} 2 & 1 \\ 3 & 1 \end{pmatrix}^{-1}
                \begin{pmatrix} 0 \\ 1 \end{pmatrix}
          =
                \frac{1}{-1}\begin{pmatrix} 1 & -1 \\ -3 & 2 \end{pmatrix}
                \begin{pmatrix} 0 \\ 1 \end{pmatrix}
                =
                \begin{pmatrix} 1 \\ -2 \end{pmatrix}.
      $$

      Therefore, $y = (1)(2x+3y) + (-2)(x+y)$.
3. WTS that $G = H_1 \oplus H_2$.
   By Problem 67.1, it suffices to show that $n(2x+3y) + m(x+y) = 0 \implies n = m = 0$.
   Then, $(2n+m)x + (3n+m)y = 0$. Since $G = \ket{x} \oplus \ket{y}$, $2n+m=0$ and $3n+m=0$. Thus, $n = m = 0$.

Therefore, $G = H_1 \oplus H_2$.

{: .no_toc}
#### Proof, with the typo.
Assume that $G$ is free abelian with basis $\set{x,y}$. WTS that $\set{2x+3y, x-y}$ is also a basis for $G$. Let $H_1 = \ket{2x+3y}$ and $H_2 = \ket{x-y}$.

1. As with the previous proof, $H_1$ and $H_2$ are both infinite cyclic groups.
2. Define a group $H = H_1 + H_2$. By Problem 67.1, $H = H_1 \oplus H_2$. Define a map $h: G \to H$ by

   $$ g = (rx, sy) \mapsto (5rx, 5sy). $$

   We need to show that $h$ is well-defined and $h$ is an isomorphism.
3. To show that $h$ is well-defined, it suffices to show that $5x, 5y$ are in the span of $\set{2x+3y, x-y}$.
   1. Let $r, s \in \Z$ with $(r)(2x+3y) + (s)(x-y) = 5x$.
      Then,

      $$
          (2r+s)x + (3r-s)y = 5x
          \implies
                \begin{pmatrix} 2 & 1 \\ 3 & -1 \end{pmatrix}
                \begin{pmatrix} r \\ s \end{pmatrix}
                =
                \begin{pmatrix} 5 \\ 0 \end{pmatrix}
          \\ \implies
                \begin{pmatrix} r \\ s \end{pmatrix}
                =
                \begin{pmatrix} 2 & 1 \\ 3 & -1 \end{pmatrix}^{-1}
                \begin{pmatrix} 5 \\ 0 \end{pmatrix}
          =
                \frac{1}{5}\begin{pmatrix} 1 & 1 \\ 3 & -2 \end{pmatrix}
                \begin{pmatrix} 5 \\ 0 \end{pmatrix}
                =
                \begin{pmatrix} 1 \\ 3 \end{pmatrix}.
      $$

   2. Let $r, s \in \Z$ with $(r)(2x+3y) + (s)(x-y) = 5y$.
      Then,

      $$
          (2r+s)x + (3r-s)y = 5y
          \implies
                \begin{pmatrix} 2 & 1 \\ 3 & -1 \end{pmatrix}
                \begin{pmatrix} r \\ s \end{pmatrix}
                =
                \begin{pmatrix} 0 \\ 5 \end{pmatrix}
          \\ \implies
                \begin{pmatrix} r \\ s \end{pmatrix}
                =
                \begin{pmatrix} 2 & 1 \\ 3 & -1 \end{pmatrix}^{-1}
                \begin{pmatrix} 0 \\ 5 \end{pmatrix}
          =
                \frac{1}{5}\begin{pmatrix} 1 & 1 \\ 3 & -2 \end{pmatrix}
                \begin{pmatrix} 0 \\ 5 \end{pmatrix}
                =
                \begin{pmatrix} 1 \\ -2 \end{pmatrix}.
      $$

    Therefore, $5x, 5y$ are in the span of $\set{2x+3y, x-y}$.

<div class='problem_issue' markdown='1'>
I can't seem to show that $h: G \to H$ is an isomorphism since I don't know if $H = \ket{5x, 5y}$.
</div>

</div>

---

<div class='problem_stmt has_issues' markdown='1'>

### Problem 67.4
The **order** of an element $a$ of an abelian group $G$ is the smallest positive integer $m$ such that $ma = 0$, if such exists; otherwise, the order of $a$ is said to be infinite. The order of $a$ thus equals the order of the subgroup generated by $a$.
{: .remove-bottom-margin}
1. Show the elements of finite order in $G$ form a subgroup of $G$ called its **torsion subgroup**.
2. Show that if $G$ is free abelian, it has no elements of finite order.
   <div class='problem_issue' markdown='1'>
   There might be a typo here. Since $G$ is a group, the identity element $1 \in G$ exists. That has order $1$. A more correct version would be: ... it has no non-trivial elements of finite order.
   </div>
3. Show the additive group of rationals has no elements of finite order, but is not free abelian. *[Hint: If $\set{a_\alpha}$ is a basis, express $\frac{1}{2}a_\alpha$ in terms of this basis.]*
{: .lower-alpha}

{: .no_toc}
#### Part (a).

{: .mt-3}
<div class='problem_notes' markdown='1'>

Recall the subgroup criterion. Given a non-empty subset $A$ of a group $G$ is a subgroup if for all $x,y \in A$, $xy^{-1} \in A$. In the case of abelian groups, check $x-y \in A$.

</div>

Let $A = \set{x \in G: |x| < \infty}$.
Let $x, y \in A$. Then, there exist $n, m \in \N$ such that $nx = my = 0$. Then, $(nm)(x-y) = nmx - nmy = m(nx) - n(my) = 0$. Therefore, $A$ is a subgroup and we'll denote it as the torsion subgroup.

{: .no_toc}
#### Part (b).
Assume $G$ is free abelian with basis $\set{x_\alpha}_{\alpha \in J}$ and suppose,
FTSOC, that there exists $x \in G \setminus \set{0}$ such that $|x| = m$. Since, by definition, $G$ is the direct sum of the infinite cyclic groups generated by the basis,

$$ x = \sum_{i=1}^{n}{a_ix_{\alpha_i}} $$

for unique $a_i \in \Z$ for all $i = 1, \dots, n$.
Then,

$$ mx = 0 = \sum_{i=1}^{n}{ma_ix_{\alpha_i}}. $$

Since $G$ is free abelian and $m \neq 0$, $ma_i = 0$ and equivalently, $a_i = 0$ for all $i = 1, \dots n$.
Therefore, $x = 0$ and $|x| = 1$. Contradiction.

{: .no_toc}
#### Part (c)(1).
Show that the additive group of rationals $(\Q,+)$ has no *non-trivial(?)* elements of finite order.

Suppose, for the sake of contradiction, that there exists $q = \frac{a}{b} \in \Q \setminus \set{0}$ such that $\abs{q} = m$ for some $m \in \N$. Then,

$$mq = m\frac{a}{b} = 0 \implies a = 0 \implies q=0. $$

Contradiction.

{: .no_toc}
#### Part (c)(2).
Suppose, FTSOC, that $(\Q,+)$ is a free abelian group. Then, there exists a basis $\set{q_\alpha}\_{\alpha \in J} \subset \Q\setminus\set{0}$ such that $\Q = \sum_{\alpha \in J}\ket{a_\alpha}$. That is, for all $q \in Q$,

$$ q = \sum_{\alpha \in J}{m_\alpha{q}_\alpha} $$

for some $m_\alpha \in \Z$ for all $\alpha \in J$. \\
<span class='comment'>Observe that for all $\alpha \in J$, $\ket{q_\alpha}$ is infinite cyclic by part (1).</span>

Fix $\beta \in J$. Then, $q_\beta \in Q$ and $\frac{1}{2}q_\beta \in \Q$. We want to represent $\frac{1}{2}q_\beta$ as a sum. Then,

$$
\begin{align*}
\frac{1}{2}q_\beta &= \sum_{\alpha \in J}{m_\alpha{q}_\alpha} \\
q_\beta &= \sum_{\alpha \in J}{2m_\alpha{q}_\alpha}.
\end{align*}
$$

Since $G$ is a direct sum, $2m_\alpha = 0$ for all $\alpha \neq \beta$ and $2m_\beta = 1$. However, this means that $m_\beta = \frac{1}{2} \not\in \Z$. Contradiction.

</div>

---

<div class='problem_stmt completed' markdown='1'>

### Problem 67.5
Give an example of a free abelian group $G$ of rank $n$ having a subgroup $H$ of rank $n$ for which $H \neq G$.

{: .no_toc}
#### Answer.
Observe that $\Z$ is a free abelian group with basis $\set{1}$ and rank $1$. Also, $2\Z \leq \Z$ is a free abelian group with basis $\set{2}$ and rank $1$. However, $\Z \neq 2\Z$.
</div>

---

<div class='problem_stmt in_progress' markdown='1'>

### Problem 67.6
**Theorem.** If $A$ is a free abelian group of rank $n$, then any subgroup $B$ of $A$ is a free abelian group of rank at most $n$.

**Proof.** We can assume $A = \Z^n$, the $n$-fold cartesian product of $\Z$ with itself. Let $\pi_i: \Z^n \to \Z$ be a projection on the $i$th coordinate. Given $m \leq n$, let $B_m$ consist of all elements $x \in B$ such that $\pi_i(x) = 0$ for $i > m$. Then, $B_m$ is a subgroup of $B$.

Consider the subgroup $\pi_m(B_m)$ of $\Z$. If this subgroup is non-trivial, choose $x_m \in B_m$ so that $\pi_m(x_m)$ is a generator of this subgroup. Otherwise, set $x_m = 0$

Prove the following:
{: .remove-bottom-margin}
1. Show that $\set{x_1, \dots, x_m}$ generates $B_m$ for each $m$.
2. Show the nonzero elements of $\set{x_1, \dots, x_n}$ form a basis for $B_m$, for each $m$.
3. Show that $B_n = B$ is free abelian with rank at most $n$.
{: .lower-alpha}

{: .no_toc}
#### Part (-1).
Assume $A$ is a free abelian group of rank $n$. Then, there exists a basis $\set{a_i}_{i=1}^{n}$ for $A$. Then, we can define a map $f: A \to \Z^n$ by

$$ x = \sum_{i=1}^{n}k_ia_i \mapsto (k_1, \dots, k_n). $$

Then, $f$ is an isomorphism.

{: .no_toc}
#### Part (0).
Continue the proof with $A \isom \Z^n$. Let $B \leq A = \Z^n$ subgroup.

For $i \in \set{1, \dots, n}$, define the map $\pi_i: \Z^n \to \Z$ as the projection on the $i$-th coordinate.

Fix $m \leq n$. Define $B_m$ as

$$ B_m = \set{x \in B \subset \Z^n : \forall i > m, \pi_i(x) = 0 }. $$

Then, $B_m$ is a subgroup of $B$.
<div class='problem_notes' markdown='1'>
Let $x, y \in B_m$. Then, $x = (x_1, x_2, \dots, x_m, 0, 0, \dots, 0)$ and $y = (y_1, y_2, \dots, y_m, 0, 0, \dots, 0)$. So,

$$
  (x-y) = (x_1 - y_1, x_2 - y_2, \dots, x_m - y_m, 0, 0, \dots, 0).
$$

For all $i > m$, $\pi_i(x-y) = 0$. Therefore, $x-y \in B_m$ and by the subgroup criterion, $B_m \leq B$.
</div>

Since [homomorphisms preserves subgroups](https://proofwiki.org/wiki/Group_Homomorphism_Preserves_Subgroups), $\pi_m(B_m)$ is a subgroup of $\Z$. Since $\Z$ is infinite cyclic and all of its [non-trivial subgroups are infinite cyclic](https://proofwiki.org/wiki/Subgroup_of_Infinite_Cyclic_Group_is_Infinite_Cyclic_Group), $\pi_m(B_m)$ has a generator, say, $x_m$. If $\pi_m(B_m)$ is trivial, set $x_m = 0$. Either way, $\pi_m(B_m) = \ket{x_m}$.

{: .no_toc}
#### Part (1).
Fix $m \leq n$. WTS that $\set{x_1, \dots, x_m}$ generate $B_m$ using induction.

For the base case, let $k=1$. Then,

$$ \begin{align*}
B_1 &= \set{a \in B \leq \Z^n : \forall i \geq 2, \pi_i(a) = 0} \\
    &= \set{a = (a_1, \dots, a_n) \isom \sum_{i=1}^n{a_i} \in B : \forall i \geq 2, a_i = 0} \\
    &= \set{a_1 : a_1 \in \pi_1(B_1)} \\
    &= \set{a_1 \in \ket{x_1}} \\
    &= \ket{x_1}.
\end{align*}
$$

For the inductive case, suppose $\set{x_1, \dots, x_k}$ generate $B_k$ for some $k$ with $1 \leq k \leq m - 1$. Then,

$$ \begin{align*}
B_{k+1} &= \set{a \in B \leq \Z^n : \forall i \geq k+2, \pi_i(a) = 0} \\
  &= \set{a = (a_1, \dots, a_n) \isom \sum_{i=1}^n{a_i} \in B : \forall i \geq k+2, a_i = 0} \\
  &= \set{a \isom \sum_{i=1}^{k+1}{a_i} : a_i \in \pi_i(B_i) } \\
  &= \set{\sum_{i=1}^{k}{a_i} + a_{k+1} :
    \sum_{i=1}^{k}{a_i} \in B_k, a_{k+1} \in \pi_{k+1}(B_{k+1})
  } \\
  &= \set{A_k + a_{k+1} : A_k \in B_k, a_{k+1} \in \ket{x_{k+1}}} \\
  &= \set{A_k + a_{k+1} : A_k \in \ket{x_1, \dots, x_n}, a_{k+1} \in \ket{x_{k+1}}} \\
  &= \set{\sum_{i=1}^{k+1}{s_ix_i} : s_i \in \Z} \\
  &= \ket{x_1, \dots, x_{k+1}}.
\end{align*}
$$

<div class='problem_issue' markdown='1'>
Notation is a tad sloppy here. Correct this later.
</div>

{: .no_toc}
#### Part (2).
Show the nonzero elements of $X_m := \set{x_1, \dots, x_m}$ form a basis for $B_m$, for each $m$. We'll do this by induction again.

For the base case, fix $k = 1$. Then, $X_1 = \set{x_1}$. If $x_1 = 0$, then $B_1$ is trivial and is free abelian (vacuously) of rank 0. Assume $x_1 \neq 0$. By construction, $\ket{x_1}$ is infinite cyclic and $B_1 = \ket{x_1} \isom \Z$ is a free abelian group.

For the inductive case, fix $k \in \set{1, ..., n-1}$. Define $Z_k = \set{z_1, \dots, z_l}$ as $X_k$ with non-zero elements removed. Assume $Z_k$ is a basis for $B_k$.

WTS that $Z_{k+1}$ (defined similarly) is a basis for $B_{k+1}$.
By construction of $z_j$, $\ket{z_j}$ is infinite cyclic for $j=1, \dots, l$. By construction of $Z_{k+1}$ and from Part (1), $Z_{k+1}$ generates $B_{k+1}$.

It remains to show that this sum is direct. Using Problem 67.1, let $a_1, \dots a_l \in \Z$ be such that

$$ \sum_{i=1}^{l}{a_iz_i} = 0. $$

Observe that if $x_k = 0$, $Z_{k+1} = Z_k$ which generates a direct sum by the inductive hypothesis. Assume $x_k \neq 0$. Then, $x_k = z_l$ and $Z_k = Z_{k+1} \setminus \set{z_l}$. Since $Z_{k}$ is a basis by assumption, for all $i \in \set{1, \dots, l-1}$, $a_i = 0$. Then,

$$ a_lz_l = 0 $$.

Since $\ket{z_l}$ is infinite cyclic, $a_l = 0$. By Problem 67.1, $Z_k$ is a basis for $B_k$.

{: .no_toc}
#### Part (3).
From Parts (1) and (2) and by setting $m=n$, $B_n = B$ is free abelian with basis $Z_n$, as defined in Part (2). Observe that $Z_n$ is a subset of $\set{x_1, \dots, x_n}$. Therefore, $|Z_n| \leq n$ and rank of $B$ is at most $n$.

</div>
