---
layout: problemset_topology_munkres2e
title: Section 52 The Fundamental Group
parent: Chapter 9 The Fundamental Group
grand_parent: Topology, Munkres 2e Solutions
permalink: topology_munkres_solutions/section52
nav_order: 2
---

This section defines the fundamental group $\pi_1(X, x_0)$ of a pointed space $(X, x_0)$, the invariance of the fundamental group on choice of base point $x_0$, and the induced homomorphism $h_*: \pi_1(X, x_0) \to \pi_1(Y, y_0)$ from a continuous map $h: \pi_1(X, x_0) \to (Y, y_0)$.

* TOC
{:toc}

---

<div class='problem_stmt completed' markdown='1'>

### Problem 52.1
A subset $A$ of $\R^n$ is said to be *star-convex* if for some point $a_0$ of $A$, all the line segments joining $a_0$ to other points of $A$ lie in $A$.
{: .remove-bottom-margin}
1. Find a star convex set that is not convex.
2. Show that if $A$ is star convex, $A$ is simply-connected.
{: .lower-alpha}

{: .no_toc}
#### Part (a).
Let $n=2$ and consider the set $A = \set{x\text{-axis}} \cup \set{y\text{-axis}}$. Fix $a_0 = (0,0)$. Then,
1. For any point $(x,0) \in \set{x\text{-axis}}$, the straight-line path $\alpha: I \to A$ from $(0,0)$ to $(x,0)$ is defined by $t \mapsto (tx, 0)$.
2. For any point $(0,y) \in \set{y\text{-axis}}$, the straight line path $\beta: I \to A$ from $(0,0)$ to $(0,y)$ is given by $t \mapsto (0, ty)$.
Observe that both images of both paths are in $A$.
Therefore, $A$ is star-convex.

<div class='problem_notes' markdown='1'>
Observe that any [regular star polygon](https://en.wikipedia.org/wiki/Star_polygon) (maybe even non-regular star polygons, if there exists a formal definition) on $\R^n$ would work with the center being $a_0$. Probably where the name 'star-convex' comes from.
</div>


{: .no_toc}
#### Part (b).
Assume $A \subset \R^n$ is star-convex with $a_0 \in A$ as described above.
Let $[f] \in \pi_1(A, a_0)$ with $f$ being a loop based at $a_0$.

Define $H: I \times I \to A$ by $(s,t) \mapsto (1-t)f(s) + ta_0$. Observe that this is a straight line homotopy and since $A$ is star-convex, for all $s \in I$, the line between $f(s)$ and $a_0$ is in $A$. Therefore, $f \simeq_p e_{a_0}$.

By transitivity of $\simeq_p$, $\pi_1(A, a_0) = \set{[f]} = \set{1}$ is trivial.

</div>

---

<div class='problem_stmt completed' markdown='1'>

### Problem 52.2
Let $\alpha$ be a path in $X$ from $x_0$ to $x_1$. Let $\beta$ be a path in $X$ from $x_1$ to $x_2$. Show that if $\gamma = \alpha * \beta$, then $\hat{\gamma} = \hat{\beta} \circ \hat{\alpha}$.

<div class='problem_notes' markdown='1'>
Recall that the hat function $\hat\alpha$ is the map used in Corollary 52.2. That is,

$$ \begin{align*}
    \hat\alpha: \pi_1(X, x_0) &\to \pi(X, x_1) \\
    [f] &\mapsto [\bar\alpha] * [f] * [\alpha]
\end{align*}
$$

Corollary 52.2 is the Change of Base Point Theorem.
</div>

{: .no_toc}
#### Proof.
Recall that the maps $\hat\alpha$ and $\hat\beta$ are defined as follows:

$$ \begin{align*}
    \hat\alpha: \pi_1(X, x_0) &\to \pi(X, x_1) \\
    [f] &\mapsto [\bar\alpha] * [f] * [\alpha]  \\
    \hat\beta: \pi_1(X, x_1) &\to \pi(X, x_2) \\
    [g] &\mapsto [\bar\beta] * [g] * [\beta]
\end{align*}
$$

Define $\gamma = \alpha * \beta$ and let $\hat\gamma$ be as follows:

$$ \begin{align*}
    \hat\gamma: \pi_1(X, x_0) &\to \pi(X, x_2)   \\
    [h] &\mapsto [\bar\gamma] * [h] * [\gamma]   
\end{align*}
$$

Let $[f] \in \pi_1(X, x_0)$.
Then,

$$ \begin{align*}
(\hat\beta \circ \hat\alpha)([f])
  &= \hat\beta(\hat\alpha([f])) \\
  &= \hat\beta( [\bar\alpha] * [f] * [\alpha] ) \\
  &= [\bar\beta] * ( [\bar\alpha] * [f] * [\alpha] ) * [\beta] \\
  &\overset{\text{Thm } 51.2}{=}
    ([\bar\beta] * [\bar\alpha]) * [f] * ([\alpha] * [\beta]) \\
  &= [\bar\beta * \bar\alpha] * [f] * [\alpha * \beta] \\
  &= [\bar\gamma] * [f] * [\gamma] \\
  &= \hat\gamma([f]).
\end{align*}
$$

</div>

---

<div class='problem_stmt completed' markdown='1'>

### Problem 52.3
Let $x_0$ and $x_1$ be points of a path-connected space $X$. Show that $\pi_1(X, x_0)$ is abelian if and only if for every pair $\alpha$ and $\beta$ of paths from $x_0$ to $x_1$, we have $\hat{\alpha} = \hat{\beta}$.

{: .no_toc}
#### Part (a). Proof.
For the forward direction, assume $\pi_1(X, x_0)$ is abelian.
Let $\alpha, \beta: I \to X$ be paths from $x_0$ to $x_1$. WTS that $\hat\alpha = \hat\beta$. <span class='note'> See Problem 52.2 for definition of $\hat\alpha$; or consult the textbook. </span>

Let $[f] \in \pi_1(X, x_0)$.
Then,

$$ \begin{align*}
    \hat\alpha([f]) = \hat\beta([f)])
    \iff& [\bar\alpha] * [f] * [\alpha] = [\bar\beta] * [f] * [\beta] \\
    \overset{\text{left mult. by } [\alpha]}{\iff}&
      [f] * [\alpha] = [\alpha] * [\bar\beta] * [f] * [\beta] \\
    \overset{\text{right mult. by } [\bar\beta]}{\iff}&
      [f] * [\alpha] * [\bar\beta] = [\alpha] * [\bar\beta] * [f] \\
    \iff&
      [f] * [\alpha * \bar\beta] = [\alpha * \bar\beta] * [f] &(*)
\end{align*}
$$

Observe that $\alpha * \bar\beta$ is a loop based at $x_0$. Then, $[\alpha * \bar\beta] \in \pi_1(X, x_0)$. Recall, by assumption, that $\pi_1(X, x_0)$ is abelian. Therefore, $(*)$ is true. Following the chain of bijections, $\hat\alpha = \hat\beta$.

{: .no_toc}
#### Part (b). Proof.
For the backwards direction, assume that for all paths $\alpha, \beta$ from $x_0$ to $x_1$, $\hat\alpha = \hat\beta$. WTS that $\pi_1(X, x_0)$ is abelian.

Let $[f], [g] \in \pi_1(X, x_0)$. WTS that $[f] * [g] = [g] * [f]$.

Let $\gamma: I \to X$ be a path from $x_0$ to $x_1$, which exists since $X$ is path-connected. Then, $g * \gamma$ is a path from $x_0$ to $x_1$. By assumption, $\hat\gamma = \widehat{g * \gamma}$. Then,

$$\begin{align*}
  \gamma([f])
    &= [\bar\gamma] * [f] * [\gamma] \\
    &= \widehat{g * \gamma}([f]) \\
    &= [\bar\gamma * \bar{g}] * [f] * [g * \gamma] \\
    &= [\bar\gamma] * [\bar{g}] * [f] * [g] * [\gamma]
\end{align*}
$$

Then,

$$\begin{align*}
  [\bar\gamma] * [f] * [\gamma] &= [\bar\gamma] * [\bar{g}] * [f] * [g] * [\gamma] \\
  [f] &= [\bar{g}] * [f] * [g] \\
  [g] * [f] = [f] * [g].
\end{align*}
$$

Therefore, $\pi_1(X, x_0)$ is abelian.

</div>

---

<div class='problem_stmt completed' markdown='1'>

### Problem 52.4
Let $A \subset X$. Suppose $r: X \to A$ is a continuous map such that $r(a) = a$ for each $a \in A$. *(The map $r$ is called a retraction of $X$ onto $A$.)* If $a_0 \in A$, show that

$$ r_* : \pi_1(X, a_0) \to \pi_1(A, a_0) $$

is surjective.

<div class='problem_notes' markdown='1'>
Recall that every function with a right inverse is surjective. For reference, check [this](https://math.stackexchange.com/questions/790274/prove-if-f-has-a-right-inverse-function-f-circ-g-id-x-iff-f-is-onto-y). While it's not needed -- also recall that every function with a left inverse is injective.
</div>

{: .no_toc}
#### Proof.
Fix $a_0 \in A$.
Let $i: A \to X$ be the inclusion map and consider its induced map, $i_*: \pi_1(A, a_0) \to \pi_1(X, a_0)$.
Then, by Theorem 52.4,

$$ r_* \circ i_* = (r \circ i)_* = (id_A)_* $$

is the identity map of $\pi_1(A, a_0)$.
Therefore, $i_*$ is a right inverse of $$r_*$$ and $$r_*$$ is surjective.

</div>

---

<div class='problem_stmt completed' markdown='1'>

### Problem 52.5
Let $A$ be a subspace of $\R^n$. Let $h: (A, a_o) \to (Y, y_o)$. Show that if $h$ is extendable to a continuous map of $\R^n$ into $Y$, then $h_*$ is the trivial homomorphism (the homomorphism that maps everything to the identity element).

{: .no_toc }
#### Proof.
Assume that $h$ extends to a continuous map $k: (\R^n, a_0) \to (Y, y_0)$. That is, for all $a \in A$, $h(a) = k(a)$.

Then, since $h = k\|_A$, $h$ is continuous and Theorem 52.4 applies. Let $i: (A, a_0) \to (\R^n, a_0)$ be the inclusion map. Then, $h = k \circ i$ and

$$ h_* = (k \circ i)_* \overset{\text{Thm 52.4}}{=} k_* \circ i_*. $$

Let $[f] \in \pi_1(A, a_0)$. Observe that $i_\*: \pi_1(A, a_0) \to \pi_1(\R^n, a_0)$ and $\pi_1(\R^n, a_0) = \set{[e_{a_0}]}$ is trivial. Also, recall that $h_*$ is a homomorphism and that is maps identity elements to identity elements.
Then,

$$
\begin{align*}
h_*([f]) &= (k_{*} \circ i_{*})([f]) \\
  &= k_\star(i_\star([f])) \\
  &= k_\star([e_{a_0}]) \\
  &= [e_{y_0}].
\end{align*}
$$

Therefore, $h_\star$ is trivial.

</div>

---

<div class='problem_stmt in_progress' markdown='1'>

### Problem 52.6

![diagram 52.6](/assets/images_tm2e/q52.6diagram.png){: width='250px'}

</div>

---

<div class='problem_stmt in_progress' markdown='1'>

### Problem 52.7

</div>
